CertiGC/bitwise_encoding.v
@@ -1,0 +1,264 @@
+Require Import VST.msl.Extensionality.
+Require Import RamifyCoq.CertiGC.bounded_numbers.
+Require Import ZArith.
+
+Open Local Scope Z.
+
+Lemma two_power_nat_pos: forall n,
+  0 < two_power_nat n.
+Proof.
+  intro. rewrite two_power_nat_equiv. rewrite <- two_p_equiv.
+  generalize (two_p_gt_ZERO (Z.of_nat n)); omega.
+Qed.
+
+Lemma two_power_nat_nonneg: forall n,
+  0 <= two_power_nat n.
+Proof. intro. generalize (two_power_nat_pos n). omega. Qed.
+
+Lemma two_power_nat_pos': forall n,
+  two_power_nat n > 0.
+Proof. intro. generalize (two_power_nat_pos n). omega. Qed.
+
+Lemma two_power_nat_lt: forall n m,
+  (n < m)%nat ->
+  two_power_nat n < two_power_nat m.
+Proof.
+  induction n; intros.
+  * destruct m. inversion H.
+    unfold two_power_nat at 1. simpl.
+    rewrite two_power_nat_S.
+    generalize (two_power_nat_pos m).
+    omega.
+  * destruct m. omega.
+    assert (n < m)%nat by omega.
+    specialize (IHn m H0).
+    do 2 rewrite two_power_nat_S. omega.
+Qed.
+
+Lemma two_power_nat_le: forall n m,
+  (n <= m)%nat ->
+  two_power_nat n <= two_power_nat m.
+Proof.
+  intros.
+  assert (n < m \/ n = m)%nat by omega.
+  destruct H0. apply two_power_nat_lt in H0. omega.
+  subst. reflexivity.
+Qed.
+
+Lemma two_power_nat_exp: forall a b,
+  two_power_nat (a + b) = two_power_nat a * two_power_nat b.
+Proof.
+  intros.
+  repeat (rewrite two_power_nat_equiv; rewrite <- two_p_equiv).
+  rewrite Nat2Z.inj_add, two_p_is_exp; omega.
+Qed.
+
+Class tagcode (A : Type) : Type := {
+  tag_bitsize : nat;
+  tag_encode  : A -> Z;
+  tag_decode  : Z -> A;
+  tag_encode_range  : forall a, (0 <= tag_encode a < two_power_nat tag_bitsize);
+  tag_decode_encode : forall a, tag_decode (tag_encode a) = a
+}.
+Implicit Arguments tag_bitsize [A].
+Implicit Arguments tag_encode [A].
+Implicit Arguments tag_decode [A].
+Implicit Arguments tag_encode_range [A].
+Implicit Arguments tag_decode_encode [A].
+
+Program Definition tag_boundZ (n : nat) : tagcode (boundZ n) :=
+  Build_tagcode (boundZ n) n (fun bz => proj1_sig bz) 
+                             (fun i => exist _ (Z.modulo i (two_power_nat n)) (Z_mod_lt _ _ (two_power_nat_pos' _))) _ _.
+Next Obligation.
+  destruct a. auto.
+Qed.
+Next Obligation.
+  destruct a. simpl. apply exist_ext. rewrite Zmod_small; omega.
+Defined.
+
+(* In the encoding, A goes on the left in the encoding *)
+Program Definition tag_prod {A} {B} (tcA : tagcode A) (tcB : tagcode B) : tagcode (A * B) :=
+  Build_tagcode (A * B) (tag_bitsize tcA + tag_bitsize tcB)
+    (fun p => ((tag_encode tcA (fst p)) * two_power_nat (tag_bitsize tcB)) + 
+                tag_encode tcB (snd p))
+    (fun i => (tag_decode tcA (i  /  two_power_nat (tag_bitsize tcB)), 
+               tag_decode tcB (i mod two_power_nat (tag_bitsize tcB)))) _ _.
+Next Obligation.
+  simpl.
+  generalize (tag_encode_range tcA a). generalize (tag_encode_range tcB b).
+  remember (tag_encode tcA a). remember (tag_encode tcB b).
+  remember (tag_bitsize tcA). remember (tag_bitsize tcB). clear.
+  split.
+  + change 0 with (0 * two_power_nat n0 + 0).
+    apply Zplus_le_compat.
+    apply Zmult_le_compat_r.
+    tauto. 
+    apply two_power_nat_nonneg.
+    tauto.
+  + rewrite two_power_nat_exp.
+    replace (two_power_nat n * two_power_nat n0) with
+            (((two_power_nat n) - 1) * two_power_nat n0 + two_power_nat n0)
+             by ring.
+    apply Zplus_le_lt_compat.
+    apply Zmult_le_compat; omega.
+    tauto.
+Qed.
+Next Obligation.
+  intros. generalize (two_power_nat_pos (tag_bitsize tcB)); intro.
+  simpl. f_equal.
+  + rewrite Z.add_comm, Z_div_plus_full, Zdiv_small, Z.add_0_l.
+    apply tag_decode_encode.
+    apply tag_encode_range.
+    omega.
+  + rewrite Zplus_mod, Z_mod_mult, Z.add_0_l, Z.mod_mod, Zmod_small.
+    apply tag_decode_encode.
+    apply tag_encode_range.
+    omega.
+Qed.
+
+Class section_retraction (A B : Type) : Type := {
+  sr_f : A -> B;
+  sr_g : B -> A;
+  sr_eq : forall b, sr_f (sr_g b) = b
+}.
+
+Program Definition tag_section_retraction {A B} (tcA: tagcode A) (srAB : section_retraction A B) : tagcode B :=
+  Build_tagcode B (tag_bitsize tcA) (fun b => tag_encode tcA (sr_g b)) 
+                                    (fun z => sr_f (tag_decode tcA z)) _ _.
+Next Obligation.
+  apply tag_encode_range.
+Qed.
+Next Obligation.
+  rewrite tag_decode_encode.
+  apply sr_eq.
+Qed.
+
+Program Definition sr_unit_boundZ (n : nat) : section_retraction (boundZ n) unit :=
+  Build_section_retraction (boundZ n) unit 
+    (fun _ => tt)
+    (fun _ => 0) _.
+Next Obligation.
+  generalize (two_power_nat_pos n).
+  omega.
+Qed.
+Next Obligation.
+  destruct b.
+  trivial.
+Qed.
+
+
+
+Definition tag_unit (n : nat) : tagcode unit := 
+  tag_section_retraction (tag_boundZ n) (sr_unit_boundZ n).
+
+Definition 
+
+  apply exist_ext.
+Lemma two_power_nat_pos: forall n,
+  0 < two_power_nat n.
+  
+
+Program Definition sr_bool_boundZ : section_retraction bool (boundZ 1) :=
+  Build_section_retraction bool (boundZ 1) 
+    (fun b => if b then 1 else 0) 
+    (fun z => if Z.eq_dec z 1 then true else false) _.
+Next Obligation.
+  unfold two_power_nat. simpl. omega.
+Qed.
+Next Obligation.
+  unfold two_power_nat. simpl. omega.
+Qed.
+Next Obligation.
+  destruct b; case Z.eq_dec; simpl; repeat intro.
+  subst. apply exist_ext. trivial.
+  apply exist_ext.
+  unfold two_power_nat in a. simpl in a. omega.
+Qed.
+
+
+
+Program Definition tag_bool : tagcode bool :=
+  Build_tagcode bool 1 (fun b => if b then 1 else 0) 
+                       (fun i => if Z.eq_dec i 1 then true else false) _ _.
+Next Obligation.
+  destruct a; unfold two_power_nat; simpl; omega.
+Qed.
+Next Obligation.
+  destruct a; auto.
+Qed.
+
+Program Definition unit_tc (n : nat) : tagcode unit :=
+  Build_tagcode unit n (fun _ => 0) (fun _ => tt) _ _.
+Next Obligation.
+  generalize (two_power_nat_pos n); omega.
+Qed.
+Next Obligation.
+  destruct a; trivial.
+Qed.
+
+
+Obligation Tactic := intros.
+
+(* Here, in the encoding, A goes on the right in the encoding *)
+Program Definition prodswap_tc {A} {B} (tcB : tagcode B) (tcA : tagcode A) : tagcode (A * B) :=
+  let X := prod_tc tcB tcA in
+    Build_tagcode (A * B) (tc_bitsize tcA + tc_bitsize tcB) 
+                          (fun a => tc_encode X (snd a, fst a)) 
+                          (fun i => (snd (tc_decode X i), fst (tc_decode X i))) _ _.
+Next Obligation.
+  unfold X. rewrite plus_comm. apply tc_encode_range.
+Qed.
+Next Obligation.
+  unfold X. rewrite tc_decode_encode. destruct a. trivial.
+Qed.
+
+Program Definition padleft_tc {A} (n : nat) (tcA : tagcode A) : tagcode A :=
+  let X := prod_tc (unit_tc n) tcA in
+    Build_tagcode A (tc_bitsize X) 
+                    (fun a => tc_encode X (tt, a)) 
+                    (fun i => snd (tc_decode X i)) _ _.
+Next Obligation.
+  unfold X. apply tc_encode_range.
+Qed.
+Next Obligation.
+  unfold X. rewrite tc_decode_encode. trivial.
+Qed.
+
+Program Definition padright_tc {A} (n : nat) (tcA : tagcode A) : tagcode A :=
+  let X := prod_tc tcA (unit_tc n) in
+    Build_tagcode A (tc_bitsize X) 
+                    (fun a => tc_encode X (a,tt)) 
+                    (fun i => fst (tc_decode X i)) _ _.
+Next Obligation.
+  unfold X. apply tc_encode_range.
+Qed.
+Next Obligation.
+  unfold X. rewrite tc_decode_encode. trivial.
+Qed.
+
+
+Obligation Tactic := Coq.Program.Tactics.program_simpl.
+
+Lemma prod_tc_mod: forall A B (tcA : tagcode A) (tcB: tagcode B) a b, 
+  tc_encode (prod_tc tcA tcB) (a,b) mod two_power_nat (tc_bitsize tcB) = tc_encode tcB b.
+Proof.
+  intros.
+  simpl.
+  generalize (two_power_nat_pos (tc_bitsize tcB)). intro.
+  rewrite Zplus_mod, Z_mod_mult, Z.add_0_l, Z.mod_mod, Zmod_small.
+  trivial.
+  apply tc_encode_range.
+  omega.
+Qed.
+
+Lemma prod_tc_div: forall A B (tcA : tagcode A) (tcB: tagcode B) a b,
+  tc_encode (prod_tc tcA tcB) (a,b) / two_power_nat (tc_bitsize tcB) = tc_encode tcA a.
+Proof.
+  intros. simpl.
+  rewrite Z.add_comm, Z_div_plus_full, Zdiv_small, Z.add_0_l.
+  trivial.
+  apply tc_encode_range.
+  generalize (two_power_nat_pos (tc_bitsize tcB)).
+  omega.
+Qed.
+
