CertiGC/cc_bitwise_encoding.v
@@ -1,0 +1,43 @@
+Require Import RamifyCoq.CertiGC.bitwise_encoding.
+Require Import VST.floyd.proofauto.
+
+Class tagint_lossless {A : Type} (tcA : tagcode A) : Type :=
+  til_bound: (tc_bitsize tcA <= Int.wordsize)%nat.
+
+Definition int_of_tag {A : Type} `{tcA : tagcode A} : A -> int :=
+  fun a => Int.repr (tc_encode tcA a).
+
+Definition tag_of_int {A : Type} `{tcA : tagcode A} : int -> A :=
+  fun i => tc_decode tcA (Int.unsigned i).
+
+Lemma tag_of_int_of_tag {A} `{tcA : tagcode A} `{tcAl: @tagint_lossless A tcA}: forall a,
+  tag_of_int (int_of_tag a) = a.
+Proof.
+  intros.
+  red in tcAl. unfold tag_of_int, int_of_tag.
+  rewrite Int.unsigned_repr. apply tc_decode_encode.
+  generalize (tc_encode_range tcA a); intro.
+  unfold Int.max_unsigned. unfold Int.modulus.
+  apply two_power_nat_le in tcAl.
+  omega.
+Qed.
+
+Lemma int_of_tag_modu {A} {B} `{tcA : tagcode A} `{tcB : tagcode B}:
+  forall a b, Int.modu (@int_of_tag (A * B) (prod_tc tcA tcB) (a,b)) 
+                      (Int.repr (two_power_nat (tc_bitsize tcB))) =
+              int_of_tag b.
+Proof.
+  intros.
+  unfold int_of_tag. simpl.
+(* SearchAbout Int.modu. *)
+Admitted.
+
+Lemma int_of_tag_divu {A} {B} `{tcA : tagcode A} `{tcB : tagcode B}:
+  forall a b, Int.divu (@int_of_tag (A * B) (prod_tc tcA tcB) (a,b)) 
+                      (Int.repr (two_power_nat (tc_bitsize tcB))) =
+              int_of_tag a.
+Proof.
+  intros.
+  unfold int_of_tag. simpl.
+(* SearchAbout Int.divu. *)
+Admitted.
